WIP on func proof, includes isolated improvements to other levels

src/Bedrock/Proofs/Func.v
@@ -2,17 +2,22 @@ Require Import Coq.ZArith.ZArith.
 Require Import Coq.Strings.String.
 Require Import Coq.Lists.List.
 Require Import Coq.micromega.Lia.
+Require Import bedrock2.Array.
+Require Import bedrock2.Scalars.
 Require Import bedrock2.Syntax.
 Require Import bedrock2.ProgramLogic.
 Require Import bedrock2.Map.Separation.
+Require Import bedrock2.Map.SeparationLogic.
 Require Import bedrock2.WeakestPreconditionProperties.
 Require Import coqutil.Word.Interface.
 Require Import coqutil.Word.Properties.
 Require Import coqutil.Map.Interface.
 Require Import coqutil.Map.Properties.
 Require Import Crypto.Bedrock.Types.
+Require Import Crypto.Bedrock.Tactics.
 Require Import Crypto.Bedrock.Proofs.Cmd.
 Require Import Crypto.Bedrock.Proofs.Flatten.
+Require Import Crypto.Bedrock.Proofs.Varnames.
 Require Import Crypto.Bedrock.Translation.Func.
 Require Import Crypto.Bedrock.Translation.Flatten.
 Require Import Crypto.Bedrock.Translation.LoadStoreList.
@@ -45,65 +50,251 @@ Section Func.
       forall {b} e, valid_cmd e -> valid_func (t:=type.base b) e
   .
 
-  (* produces a separation-logic condition stating that the values of arguments are equivalent *)
-  (* TODO: should this go in Types.v? *)
-  Fixpoint equivalent_args {t}
-    : type.for_each_lhs_of_arrow API.interp_type t -> (* fiat-crypto value *)
-      type.for_each_lhs_of_arrow (rtype (listZ:=rep.listZ_mem)) t -> (* bedrock2 value *)
-      Semantics.locals -> Semantics.mem -> Prop :=
+  (* TODO : move *)
+  (* separation-logic relation that says space exists in memory for lists
+     (other values are ignored) *)
+  Fixpoint lists_reserved {t}
+    : base_list_lengths t ->
+      Interface.map.rep (map:=Semantics.mem) -> (* memory *)
+      Prop :=
     match t with
-    | type.base b => fun _ _ _ _ => True
-    | type.arrow (type.base a) b =>
-      fun (x : base.interp a * _) (y : base_rtype a * _) locals =>
-        sep (equivalent (fst x) (fst y) locals)
-            (equivalent_args (snd x) (snd y) locals)
-    | _ => fun _ _ _ _ => False
+    | base.type.prod a b =>
+      fun x => sep (lists_reserved (fst x)) (lists_reserved (snd x))
+    | base_listZ =>
+      fun n =>
+        Lift1Prop.ex1
+          (fun start : Semantics.word =>
+             Lift1Prop.ex1
+               (fun oldvalues : list Semantics.word =>
+                  let size := Interface.word.of_Z (Z.of_nat n) in
+                  array scalar size start oldvalues))
+    | base_Z => fun _ _ => True
+    |  _ => fun _ _ => False
     end.
 
-  (* TODO: use spec_of *)
-  Lemma translate_func_correct {t}
+  (* TODO : move *)
+  Lemma load_arguments_correct {t} :
+    forall (argnames : type.for_each_lhs_of_arrow ltype t)
+           (arglengths : type.for_each_lhs_of_arrow list_lengths t)
+           (args1 : type.for_each_lhs_of_arrow API.interp_type t)
+           (args2 : type.for_each_lhs_of_arrow rtype t)
+           (flat_args : list Semantics.word)
+           (functions : list _)
+           (tr : Semantics.trace)
+           (locals : Semantics.locals)
+           (mem : Semantics.mem)
+           (nextn : nat)
+           (R : Semantics.mem -> Prop),
+        (* argument values (in their 3 forms) are equivalent *)
+        sep (equivalent_args args1 args2 map.empty) R mem ->
+        WeakestPrecondition.dexprs
+          mem map.empty (flatten_args args2) flat_args ->
+        (* locals have just been formed from arguments *)
+        map.of_list_zip (flatten_argnames argnames) flat_args = Some locals ->
+        (* load_arguments returns triple : # fresh variables used,
+           new argnames with local lists, and cmd *)
+        let out := load_arguments nextn argnames arglengths in
+        (* translated function produces equivalent results *)
+        WeakestPrecondition.cmd
+          (WeakestPrecondition.call functions)
+          (snd out)
+          tr mem locals
+          (fun tr' mem' locals' =>
+             tr = tr' /\
+             mem = mem' /\
+             locally_equivalent_args args1 args2 locals').
+  Proof.
+  Admitted.
+
+  Search list_lengths.
+
+  (* idea: pull return list lengths from fiat-crypto type *)
+  (* TODO : move *)
+  Lemma store_return_values_correct {t} :
+    forall (retnames_local : base_ltype t)
+           (retnames_mem : base_ltype t)
+           (retlengths : base_list_lengths t)
+           (rets : base.interp t)
+           (functions : list _)
+           (tr : Semantics.trace)
+           (locals : Semantics.locals)
+           (mem : Semantics.mem)
+           (R : Semantics.mem -> Prop),
+        (* use old values of memory to set up frame for return values *)
+        sep (lists_reserved retlengths) R mem ->
+        (* rets are stored in local retnames *)
+        locally_equivalent rets (rtype_of_ltype retnames_local) locals ->
+        (* translated function produces equivalent results *)
+        WeakestPrecondition.cmd
+          (WeakestPrecondition.call functions)
+          (store_return_values retnames_local retnames_mem)
+          tr mem locals
+          (fun tr' mem' locals' =>
+             tr = tr' /\
+             sep (equivalent rets (rtype_of_ltype retnames_mem) locals') R mem').
+  Proof.
+  Admitted.
+
+  Fixpoint init_context {t} {listZ:rep.rep base_listZ}:
+    type.for_each_lhs_of_arrow API.interp_type t ->
+    type.for_each_lhs_of_arrow (ltype (listZ:=listZ)) t ->
+    list {t' & (unit * API.interp_type t' * ltype t')%type} :=
+            match t with
+            | type.base b => fun _ _ => []
+            | type.arrow (type.base a) b =>
+              fun args argnames =>
+                (existT _ (type.base a) (tt, fst args, fst argnames)
+                        :: init_context (snd args) (snd argnames))
+            | _ => fun _ _ => []
+            end.
+
+  Lemma translate_func'_correct {t}
         (* three exprs, representing the same Expr with different vars *)
         (e0 : @API.expr (fun _ => unit) t)
         (e1 : @API.expr API.interp_type t)
         (e2 : @API.expr ltype t)
+        (* expressions are valid input to translate_func' *)
+        (e0_valid : valid_func e0)
+        (* context list (consists only of arguments) *)
+        (G : list _) :
+    (* exprs are all related *)
+    wf3 G e0 e1 e2 ->
+    forall (argnames : type.for_each_lhs_of_arrow ltype t)
+           (args : type.for_each_lhs_of_arrow API.interp_type t)
+           (nextn : nat),
+      (* ret1 := fiat-crypto interpretation of e1 applied to args1 *)
+      let ret1 : base.interp (type.final_codomain t) :=
+          type.app_curried (API.interp e1) args in
+      (* out := translation output for e2; triple of
+         (# varnames used, return values, cmd) *)
+      let out := translate_func' e2 nextn argnames in
+      let nvars := fst (fst out) in
+      let ret2 := rtype_of_ltype (snd (fst out)) in
+      let body := snd out in
+      (* G doesn't contain variables we could accidentally overwrite *)
+      (forall n,
+          (nextn <= n)%nat ->
+          Forall (varname_not_in_context (varname_gen n)) G) ->
+      forall (tr : Semantics.trace)
+             (locals : Semantics.locals)
+             (mem : Semantics.mem)
+             (functions : list bedrock_func),
+        (* contexts are equivalent; for every variable in the context list G,
+             the fiat-crypto and bedrock2 results match *)
+        context_equiv G locals ->
+        (* executing translation output is equivalent to interpreting e *)
+        WeakestPrecondition.cmd
+          (WeakestPrecondition.call functions)
+          body tr mem locals
+          (fun tr' mem' locals' =>
+             tr = tr' /\
+             mem = mem' /\
+             Interface.map.only_differ
+               locals (used_varnames nextn nvars) locals' /\
+             locally_equivalent (listZ:=rep.listZ_local) ret1 ret2 locals').
+  Admitted.
+
+  (* TODO : move *)
+  Fixpoint list_lengths_from_value {t}
+    : base.interp t -> base_list_lengths t :=
+    match t as t0 return base.interp t0 -> base_list_lengths t0 with
+    | base.type.prod a b =>
+      fun x : base.interp a * base.interp b =>
+        (list_lengths_from_value (fst x),
+         list_lengths_from_value (snd x))
+    | base_listZ => fun x : list Z => length x
+    | _ => fun _ => tt
+    end.
+
+  (* TODO : move *)
+  Fixpoint list_lengths_from_args {t}
+    : type.for_each_lhs_of_arrow API.interp_type t ->
+      type.for_each_lhs_of_arrow list_lengths t :=
+    match t with
+    | type.base b => fun _ => tt
+    | type.arrow (type.base a) b =>
+      fun x =>
+        (list_lengths_from_value (fst x), list_lengths_from_args (snd x))
+    | type.arrow a b =>
+      fun x => (tt, list_lengths_from_args (snd x))
+    end.
+
+
+  (* This lemma handles looking up the return values *)
+  (* TODO : rename *)
+  Lemma look_up_return_values {t} :
+    forall (ret : base.interp t)
+           (retnames : base_ltype (listZ:=rep.listZ_mem) t)
+           (locals : Semantics.locals)
+           (mem : Semantics.mem)
+           (R : Semantics.mem -> Prop),
+    sep (equivalent ret (rtype_of_ltype retnames) locals) R mem ->
+    WeakestPrecondition.list_map
+      (WeakestPrecondition.get locals) (flatten_retnames retnames)
+      (fun flat_rets =>
+         exists ret',
+           WeakestPrecondition.dexprs mem map.empty (flatten_rets ret') flat_rets /\
+           sep (equivalent ret ret' map.empty) R mem).
+  Proof.
+    cbv [flatten_retnames].
+    induction t; cbn [flatten_base_ltype equivalent]; break_match;
+      repeat match goal with
+             | _ => progress (intros; cleanup)
+             | _ => progress subst
+             | _ => progress cbn [rep.equiv rep.listZ_mem rep.Z] in *
+             | _ => progress cbn [WeakestPrecondition.list_map WeakestPrecondition.list_map_body]
+             | H : sep (emp _) _ _ |- _ => apply sep_emp_l in H
+             | H : WeakestPrecondition.dexpr _ _ _ _ |- _ => destruct H
+             | |- WeakestPrecondition.get _ _ _ => eexists; split; [ eassumption | ]
+             end.
+    (* TODO *)
+  Admitted.
+
+  Lemma translate_func_correct {t}
+        (e : API.Expr t)
         (* expressions are valid input to translate_func *)
-        (e0_valid : valid_func e0) :
-    (* exprs are all related with empty context *)
-    wf3 [] e0 e1 e2 ->
+        (e_valid : valid_func (e _)) :
+    Wf3 e ->
     forall (fname : string)
            (retnames : base_ltype (type.final_codomain t))
            (argnames : type.for_each_lhs_of_arrow ltype t)
-           (arglengths : type.for_each_lhs_of_arrow list_lengths t)
            (args1 : type.for_each_lhs_of_arrow API.interp_type t)
            (args2 : type.for_each_lhs_of_arrow rtype t),
       (* rets1 := fiat-crypto interpretation of e1 applied to args1 *)
       let rets1 : base.interp (type.final_codomain t) :=
-          type.app_curried (API.interp e1) args1 in
-      (* out := translation output for e2 (function arguments, rets, body) *)
-      let out := translate_func e2 argnames arglengths retnames in
+          type.app_curried (API.interp (e _)) args1 in
+      (* extract list lengths from fiat-crypto arguments/return values *)
+      let arglengths := list_lengths_from_args args1 in
+      let retlengths := list_lengths_from_value rets1 in
+      (* out := translation output for e2; triple of
+         (function arguments, function return variable names, body) *)
+      let out := translate_func e argnames arglengths retnames in
       let f : bedrock_func := (fname, out) in
       forall (tr : Semantics.trace)
              (mem : Semantics.mem)
              (flat_args : list Semantics.word)
              (functions : list bedrock_func)
-             (P R : Semantics.mem -> Prop),
+             (P Ra Rr : Semantics.mem -> Prop),
         (* argument values (in their 3 forms) are equivalent *)
-        equivalent_args args1 args2 map.empty mem ->
+        sep (equivalent_args args1 args2 map.empty) Ra mem ->
         WeakestPrecondition.dexprs
           mem map.empty (flatten_args args2) flat_args ->
-        (* TODO: make P say something about having the same shape as rets *)
-        sep P R mem ->
+        (* seplogic frame for return values *)
+        sep (lists_reserved retlengths) Rr mem ->
         (* translated function produces equivalent results *)
         WeakestPrecondition.call
           ((fname, out) :: functions) fname tr mem flat_args
           (fun tr' mem' flat_rets =>
              tr = tr' /\
-             (exists rets2 : base_rtype (type.final_codomain t),
-                 WeakestPrecondition.dexprs
-                   mem map.empty (flatten_rets rets2) flat_rets /\
-                 sep (equivalent (listZ:=rep.listZ_mem) rets1 rets2 map.empty) R mem')).
+             exists rets2 : base_rtype (type.final_codomain t),
+               (* rets2 is a valid representation of flat_rets with no local
+                  variables in context *)
+               WeakestPrecondition.dexprs
+                 mem' map.empty (flatten_rets rets2) flat_rets /\
+               (* return values are equivalent *)
+               sep (equivalent (listZ:=rep.listZ_mem) rets1 rets2 map.empty) Rr mem').
   Proof.
-    cbv zeta. intros; cbv [translate_func].
+    cbv [translate_func Wf3]; intros.
     cbn [WeakestPrecondition.call WeakestPrecondition.call_body WeakestPrecondition.func].
     rewrite eqb_refl.
     match goal with H : _ |- _ =>
@@ -111,5 +302,20 @@ Section Func.
                       destruct H
     end.
     eexists; split; [ eassumption | ].
-  Admitted.
+    cbn [WeakestPrecondition.cmd WeakestPrecondition.cmd_body].
+    eapply Proper_cmd; [ solve [apply Proper_call] | repeat intro | ].
+    2 : {
+      eapply load_arguments_correct; eassumption. }
+    cbv beta in *. cleanup; subst.
+    eapply Proper_cmd; [ solve [apply Proper_call] | repeat intro | ].
+    2 : { eapply translate_func'_correct with (args:=args1); cbv [context_equiv]; eauto. }
+    cbv beta in *. cleanup; subst.
+    eapply Proper_cmd; [ solve [apply Proper_call] | repeat intro | ].
+    2 : { eapply store_return_values_correct; eauto. }
+    cbv beta in *. cleanup; subst.
+
+    eapply Proper_list_map; [ solve [apply Proper_get]
+                            | | eapply look_up_return_values; solve [eauto] ].
+    repeat intro; eauto.
+  Qed.
 End Func.
